cfrontend/BeePL_auxlemmas.v
@@ -1,7 +1,7 @@
 Require Import String ZArith Coq.FSets.FMapAVL Coq.Structures.OrderedTypeEx FunInd.
 Require Import Coq.FSets.FSetProperties Coq.FSets.FMapFacts FMaps FSetAVL Nat PeanoNat Linking.
 Require Import Coq.Arith.EqNat Coq.ZArith.Int Integers AST Maps Linking Ctypes Smallstep SimplExpr.
-Require Import BeePL_aux BeePL_mem BeeTypes BeePL Csyntax Clight Globalenvs BeePL_Csyntax SimplExpr.
+Require Import BeePL BeePL_aux BeePL_mem BeeTypes BeePL Csyntax Clight Globalenvs BeePL_Csyntax SimplExpr.
 Require Import compcert.common.Errors Initializersproof Cstrategy lib.Coqlib Errors.
 
 From mathcomp Require Import all_ssreflect. 
@@ -32,6 +32,9 @@ transC_val_bplvalue v' = OK v ->
 transBeePL_value_cvalue v = v'.
 Proof.
 Admitted.
+
+
+
 
 
 
